wip

DynamoDbEncryption/runtimes/python/src/aws_database_encryption_sdk/encryptor/client.py
@@ -1,0 +1,109 @@
+# Copyright Amazon.com Inc. or its affiliates. All Rights Reserved.
+# SPDX-License-Identifier: Apache-2.0
+"""High-level helper class to provide an encrypting wrapper for boto3 DynamoDB clients."""
+from botocore.paginate import Paginator
+import botocore.client
+from typing import Callable, Optional
+
+from aws_database_encryption_sdk.smithygenerated.aws_cryptography_dbencryptionsdk_dynamodb_transforms.models import (
+    GetItemInputTransformInput,
+    GetItemOutputTransformInput,
+    PutItemInputTransformInput,
+    PutItemOutputTransformInput,
+)
+from aws_database_encryption_sdk.transform import (
+    dict_to_ddb,
+    ddb_to_dict,
+)
+from aws_database_encryption_sdk.smithygenerated.aws_cryptography_dbencryptionsdk_dynamodb_transforms.client import (
+    DynamoDbEncryptionTransforms
+)
+from aws_database_encryption_sdk.smithygenerated.aws_cryptography_dbencryptionsdk_dynamodb.models import (
+    DynamoDbTablesEncryptionConfig,
+)
+
+
+class EncryptedClient:
+    """
+    A client that provides encryption and decryption for an underlying boto3 DynamoDB client.
+    """
+
+    _client: botocore.client.BaseClient
+    _encryption_config: DynamoDbTablesEncryptionConfig
+    _expect_standard_dictionaries: Optional[bool]
+    _transformer: DynamoDbEncryptionTransforms
+
+    def __init__(
+        self,
+        *,
+        client: botocore.client.BaseClient,
+        encryption_config: DynamoDbTablesEncryptionConfig,
+        expect_standard_dictionaries: Optional[bool] = False,
+    ):
+        """
+        Parameters:
+        client (botocore.client.BaseClient): Initialized boto3 DynamoDB client
+        encryption_config (DynamoDbTablesEncryptionConfig): Initialized DynamoDbTablesEncryptionConfig
+        expect_standard_dictionaries (Optional[bool]): Should we expect items to be standard Python
+            dictionaries? (default: False)
+        """
+        self._client = client
+        self._encryption_config = encryption_config
+        self._expect_standard_dictionaries = expect_standard_dictionaries
+        self._transformer = DynamoDbEncryptionTransforms(
+            config = encryption_config
+        )
+
+    def put_item(self, **kwargs):
+        # TODO: refactor shared logic (DDB/Python conversions)
+        if self._expect_standard_dictionaries:
+            dynamodb_item = dict_to_ddb(kwargs["Item"])
+            dynamodb_input = kwargs
+            dynamodb_input["Item"] = dynamodb_item
+        else:
+            dynamodb_input = kwargs
+        transformed_request = self._transformer.put_item_input_transform(
+            PutItemInputTransformInput(
+                sdk_input = dynamodb_input
+            )
+        ).transformed_input
+        sdk_output = self._client.put_item(**transformed_request)
+        transformed_response = self._transformer.put_item_output_transform(
+            PutItemOutputTransformInput(
+                original_input = dynamodb_input,
+                sdk_output = sdk_output,
+            )
+        ).transformed_output
+        response = transformed_response
+        for sdk_output_key, sdk_output_value in sdk_output.items():
+            if sdk_output_key not in transformed_response:
+                response[sdk_output_key] = sdk_output_value
+        # TODO: standard dicts transform output
+        return response
+    
+    def get_item(self, **kwargs):
+        if self._expect_standard_dictionaries:
+            dynamodb_item = dict_to_ddb(kwargs["Key"])
+            dynamodb_input = kwargs
+            dynamodb_input["Key"] = dynamodb_item
+        else:
+            dynamodb_input = kwargs
+        transformed_request = self._transformer.get_item_input_transform(
+            GetItemInputTransformInput(
+                sdk_input = dynamodb_input
+            )
+        ).transformed_input
+        sdk_output = self._client.get_item(**transformed_request)
+        transformed_response = self._transformer.get_item_output_transform(
+            GetItemOutputTransformInput(
+                original_input = dynamodb_input,
+                sdk_output = sdk_output,
+            )
+        ).transformed_output
+        response = transformed_response
+        for sdk_output_key, sdk_output_value in sdk_output.items():
+            if sdk_output_key not in transformed_response:
+                response[sdk_output_key] = sdk_output_value
+        if self._expect_standard_dictionaries:
+            response["Item"] = ddb_to_dict(response["Item"])
+        return response
