DynamoDbEncryption/runtimes/python/src/aws_database_encryption_sdk/encryptor/item.py
@@ -1,0 +1,187 @@
+# Copyright Amazon.com Inc. or its affiliates. All Rights Reserved.
+# SPDX-License-Identifier: Apache-2.0
+"""Top-level class for encrypting and decrypting individual DynamoDB items."""
+from typing import Optional, Dict, Any
+
+from aws_database_encryption_sdk.smithygenerated.aws_cryptography_dbencryptionsdk_dynamodb_itemencryptor.config import (
+    DynamoDbItemEncryptorConfig,
+)
+from aws_database_encryption_sdk.smithygenerated.aws_cryptography_dbencryptionsdk_dynamodb_itemencryptor.client import (
+    DynamoDbItemEncryptor,
+)
+from aws_database_encryption_sdk.smithygenerated.aws_cryptography_dbencryptionsdk_dynamodb_itemencryptor.models import (
+    DecryptItemInput,
+    DecryptItemOutput,
+    EncryptItemInput,
+    EncryptItemOutput,
+)
+from aws_database_encryption_sdk.transform import (
+    dict_to_ddb,
+    ddb_to_dict,
+)
+
+class ItemEncryptor:
+    """Client providing item-level encryption for DynamoDB items / Python dictionaries."""
+
+    _internal_client: DynamoDbItemEncryptor
+
+    def __init__(
+        self,
+        *,
+        item_encryptor_config: Optional[DynamoDbItemEncryptorConfig] = None,
+        initialized_client: Optional[DynamoDbItemEncryptor] = None,
+        expect_standard_dictionaries: Optional[bool] = False,
+    ):
+        """
+        Create an ItemEncryptor.
+        Must provide exactly one of `item_encryptor_config` or `initialized_client`.
+
+        Parameters:
+        item_encryptor_config (Optional[DynamoDbItemEncryptorConfig]): Encryption configuration object.
+        initialized_client (Optional[DynamoDbItemEncryptor]): Initialized DynamoDbItemEncryptor.
+
+        """
+        if item_encryptor_config is None and initialized_client is None:
+            raise ValueError("Must provide exactly one of item_encryptor_config or initialized_client")
+        elif item_encryptor_config is not None and initialized_client is not None:
+            raise ValueError("Must provide exactly one of item_encryptor_config or initialized_client")
+        elif item_encryptor_config is not None:
+            self._internal_client = DynamoDbItemEncryptor(config = item_encryptor_config)
+        elif initialized_client is not None:
+            self._internal_client = initialized_client
+        else:
+            raise ValueError("Unknown state for ItemEncryptor construction")
+
+    def encrypt_dynamodb_item(self, plaintext_ddb_item: Dict[str, Any]) -> EncryptItemOutput:
+        """
+        Encrypt a DynamoDB item.
+
+        boto3 DynamoDB clients expect items formatted as DynamoDB items.
+        Use this method to encrypt an item you intend to store using a boto3 DynamoDB client.
+
+        Parameters:
+        plaintext_ddb_item (Dict[str, Any]): A dictionary representing a DynamoDB item.
+        
+        Returns:
+        EncryptItemOutput: Structure containing the following fields:
+            - `encrypted_item` (dict[str, Any]): The encrypted DynamoDB item.
+            - `parsed_header` (Optional[ParsedHeader]): The encrypted DynamoDB item's header (`aws_dbe_head` value).
+
+        Example:
+        
+        >>> plaintext_item = {
+        ...     'some': {'S': 'data'},
+        ...     'more': {'N': '5'}
+        ... }
+        >>> encrypted_item = item_encryptor.encrypt_dynamodb_item(
+        ...     plaintext_ddb_item = plaintext_item
+        ... )
+        """
+        encrypt_item_output: EncryptItemOutput = self._internal_client.encrypt_item(
+            EncryptItemInput(
+                plaintext_item = plaintext_ddb_item
+            )
+        )
+        return encrypt_item_output
+
+    def encrypt_python_item(self, plaintext_dict_item: Dict[str, Any]) -> EncryptItemOutput:
+        """
+        Encrypt a Python dictionary.
+        This method will convert the Python dictionary into a DynamoDB item, then encrypt the item.
+
+        boto3 DynamoDB Tables and Resources expect items formatted as native Python dictionaries.
+        Use this method to encrypt an item you intend to store using a boto3 DynamoDB Table or Resource interface.
+
+        Parameters:
+        plaintext_dict_item (Dict[str, Any]): A standard Python dictionary.
+        
+        Returns:
+        EncryptItemOutput: Structure containing the following fields:
+            - `encrypted_item` (dict[str, Any]): The encrypted Python dictionary.
+                **Note:** The item was encrypted as a DynamoDB item, then converted back to a native Python item.
+            - `parsed_header` (Optional[ParsedHeader]): The encrypted DynamoDB item's header (`aws_dbe_head` value).
+
+        Example:
+        
+        >>> plaintext_item = {
+        ...     'some': 'data',
+        ...     'more': 5
+        ... }
+        >>> encrypted_item = item_encryptor.encrypt_python_item(
+        ...     plaintext_dict_item = plaintext_item,
+        ... )
+        """
+        plaintext_ddb_item = dict_to_ddb(plaintext_dict_item)
+        encrypted_ddb_item: EncryptItemOutput = self.encrypt_dynamodb_item(plaintext_ddb_item)
+        encrypted_dict_item = ddb_to_dict(encrypted_ddb_item.encrypted_item)
+        return EncryptItemOutput(
+            encrypted_item = encrypted_dict_item,
+            parsed_header = encrypted_ddb_item.parsed_header
+        )
+
+    def decrypt_dynamodb_item(self, encrypted_ddb_item: Dict[str, Any]) -> DecryptItemOutput:
+        """
+        Decrypt a DynamoDB item.
+
+        boto3 DynamoDB clients expect items formatted as DynamoDB items.
+        Use this method to decrypt an item you retrieved using a boto3 DynamoDB client.
+
+        Parameters:
+        encrypted_ddb_item (dict[str, Any]): A dictionary representing an encrypted DynamoDB item.
+        
+        Returns:
+        DecryptItemOutput: Structure containing the following fields:
+            - `plaintext_item` (dict[str, Any]): The plaintext DynamoDB item.
+            - `parsed_header` (Optional[ParsedHeader]): The decrypted DynamoDB item's header (`aws_dbe_head` value).
+
+        Example:
+        
+        >>> encrypted_item = {
+        ...     'some': {'B': b'ENCRYPTED_DATA'},
+        ...     'more': {'B': b'ENCRYPTED_DATA'}
+        ... }
+        >>> decrypted_item = item_encryptor.decrypt_dynamodb_item(
+        ...     encrypted_ddb_item = encrypted_item,
+        ... )
+        """
+        decrypt_item_output: DecryptItemOutput = self._internal_client.decrypt_item(
+            DecryptItemInput(
+                encrypted_item = encrypted_ddb_item
+            )
+        )
+        return decrypt_item_output
+
+    def decrypt_python_item(self, encrypted_dict_item: Dict[str, Any]) -> DecryptItemOutput:
+        """
+        Decrypt a Python dictionary.
+        This will convert the Python dictionary into a DynamoDB item, then decrypt the item.
+
+        boto3 DynamoDB Tables and Resources expect items formatted as native Python dictionaries.
+        Use this method to decrypt an item you retrieved using a boto3 DynamoDB Table or Resource interface.
+
+        Parameters:
+        encrypted_dict_item (Dict[str, Any]): A standard Python dictionary with encrypted values.
+        
+        Returns:
+        DecryptItemOutput: Structure containing the following fields:
+            - `encrypted_item` (dict[str, Any]): The decrypted Python dictionary.
+                **Note:** The item was decrypted as a DynamoDB item, then converted back to a native Python item.
+            - `parsed_header` (Optional[ParsedHeader]): The decrypted DynamoDB item's header (`aws_dbe_head` value).
+
+        Example:
+        
+        >>> plaintext_item = {
+        ...     'some': 'data',
+        ...     'more': 5
+        ... }
+        >>> encrypted_item = item_encryptor.encrypt_python_item(
+        ...     plaintext_dict_item = plaintext_item,
+        ... )
+        """
+        encrypted_ddb_item = dict_to_ddb(encrypted_dict_item)
+        plaintext_ddb_item: DecryptItemOutput = self.decrypt_dynamodb_item(encrypted_ddb_item)
+        plaintext_dict_item = ddb_to_dict(plaintext_ddb_item.plaintext_item)
+        return DecryptItemOutput(
+            plaintext_item = plaintext_dict_item,
+            parsed_header = plaintext_ddb_item.parsed_header
+        )
