DynamoDbEncryption/runtimes/python/src/aws_database_encryption_sdk/smithygenerated/aws_cryptography_dbencryptionsdk_dynamodb/errors.py
@@ -3,7 +3,7 @@
 # Do not modify this file. This file is machine generated, and any changes to it will be overwritten.
 
 import _dafny
-from aws_cryptographic_materialproviders.smithygenerated.aws_cryptography_materialproviders.errors import (
+from aws_cryptographic_material_providers.smithygenerated.aws_cryptography_materialproviders.errors import (
     _smithy_error_to_dafny_error as aws_cryptography_materialproviders_smithy_error_to_dafny_error,
 )
 from aws_cryptography_internal_dynamodb.smithygenerated.com_amazonaws_dynamodb.shim import (
@@ -214,6 +214,64 @@ class OpaqueError(ApiError[Literal["OpaqueError"]]):
         return all(getattr(self, a) == getattr(other, a) for a in attributes)
 
 
+class OpaqueWithTextError(ApiError[Literal["OpaqueWithTextError"]]):
+    code: Literal["OpaqueWithTextError"] = "OpaqueWithTextError"
+    obj: Any  # As an OpaqueWithTextError, type of obj is unknown
+    obj_message: str  # obj_message is a message representing the details of obj
+
+    def __init__(self, *, obj, obj_message):
+        super().__init__("")
+        self.obj = obj
+        self.obj_message = obj_message
+
+    def as_dict(self) -> Dict[str, Any]:
+        """Converts the OpaqueWithTextError to a dictionary.
+
+        The dictionary uses the modeled shape names rather than the
+        parameter names as keys to be mostly compatible with boto3.
+        """
+        return {
+            "message": self.message,
+            "code": self.code,
+            "obj": self.obj,
+            "obj_message": self.obj_message,
+        }
+
+    @staticmethod
+    def from_dict(d: Dict[str, Any]) -> "OpaqueWithTextError":
+        """Creates a OpaqueWithTextError from a dictionary.
+
+        The dictionary is expected to use the modeled shape names rather
+        than the parameter names as keys to be mostly compatible with
+        boto3.
+        """
+        kwargs: Dict[str, Any] = {
+            "message": d["message"],
+            "obj": d["obj"],
+            "obj_message": d["obj_message"],
+        }
+
+        return OpaqueWithTextError(**kwargs)
+
+    def __repr__(self) -> str:
+        result = "OpaqueWithTextError("
+        result += f"message={self.message},"
+        if self.message is not None:
+            result += f"message={repr(self.message)}"
+        result += f"obj={self.obj}"
+        result += f"obj_message={self.obj_message}"
+        result += ")"
+        return result
+
+    def __eq__(self, other: Any) -> bool:
+        if not isinstance(other, OpaqueWithTextError):
+            return False
+        if not (self.obj == other.obj):
+            return False
+        attributes: list[str] = ["message", "message"]
+        return all(getattr(self, a) == getattr(other, a) for a in attributes)
+
+
 def _smithy_error_to_dafny_error(e: ServiceError):
     """Converts the provided native Smithy-modeled error into the corresponding
     Dafny error."""
@@ -258,6 +316,11 @@ def _smithy_error_to_dafny_error(e: ServiceError):
     if isinstance(e, OpaqueError):
         return aws_database_encryption_sdk.internaldafny.generated.AwsCryptographyDbEncryptionSdkDynamoDbTypes.Error_Opaque(
             obj=e.obj
+        )
+
+    if isinstance(e, OpaqueWithTextError):
+        return aws_database_encryption_sdk.internaldafny.generated.AwsCryptographyDbEncryptionSdkDynamoDbTypes.Error_OpaqueWithText(
+            obj=e.obj, objMessage=e.obj_message
         )
 
     else:
