DynamoDbEncryption/runtimes/python/src/aws_database_encryption_sdk/smithygenerated/aws_cryptography_dbencryptionsdk_dynamodb_transforms/client.py
@@ -630,7 +630,11 @@ class DynamoDbEncryptionTransforms:
             transport_request=None,
             transport_response=None,
         )
-        _client_interceptors = config.interceptors
+        try:
+            _client_interceptors = config.interceptors
+        except AttributeError:
+            config.interceptors = []
+            _client_interceptors = config.interceptors
         client_interceptors = cast(
             list[Interceptor[Input, Output, DafnyRequest, DafnyResponse]],
             _client_interceptors,
