DynamoDbEncryption/runtimes/python/src/aws_database_encryption_sdk/smithygenerated/aws_cryptography_dbencryptionsdk_dynamodb_transforms/deserialize.py
@@ -333,6 +333,8 @@ def _deserialize_resolve_attributes(input: DafnyResponse, config: Config):
 def _deserialize_error(error: Error) -> ServiceError:
     if error.is_Opaque:
         return OpaqueError(obj=error.obj)
+    elif error.is_OpaqueWithText:
+        return OpaqueErrorWithText(obj=error.obj, obj_message=error.objMessage)
     elif error.is_CollectionOfErrors:
         return CollectionOfErrors(
             message=_dafny.string_of(error.message),
