DynamoDbEncryption/runtimes/python/src/aws_database_encryption_sdk/transform.py
@@ -1,0 +1,32 @@
+# Copyright Amazon.com Inc. or its affiliates. All Rights Reserved.
+# SPDX-License-Identifier: Apache-2.0
+"""Helper tools for translating between native and DynamoDB items.
+
+For information on how types are serializes, see:
+https://boto3.amazonaws.com/v1/documentation/api/latest/_modules/boto3/dynamodb/types.html
+"""
+from typing import Any, Dict
+
+from boto3.dynamodb.types import TypeDeserializer, TypeSerializer
+
+__all__ = ("dict_to_ddb", "ddb_to_dict")
+
+
+def dict_to_ddb(item: Dict[str, Any]) -> Dict[str, Any]:
+    """Converts a native Python dictionary to a raw DynamoDB item.
+
+    :param dict item: Native item
+    :returns: DynamoDB item
+    """
+    serializer = TypeSerializer()
+    return {key: serializer.serialize(value) for key, value in item.items()}
+
+
+def ddb_to_dict(item: Dict[str, Any]) -> Dict[str, Any]:
+    """Converts a raw DynamoDB item to a native Python dictionary.
+
+    :param dict item: DynamoDB item
+    :returns: Native item
+    """
+    deserializer = TypeDeserializer()
+    return {key: deserializer.deserialize(value) for key, value in item.items()}
